Kura/Operation/VxIdentification.lean
@@ -1,0 +1,54 @@
+import Kura.Operation.MapHom
+
+
+open Set Function
+variable {α α' α'' β β' : Type*} {G H : Graph (Set α) β} {a b c : α} {x y z : Set α} {e f : β}
+
+namespace Graph
+
+/- I have been thinking about a way to `contract` without supplying the vx map but just the edge
+set I am contracting on. This is one way to do it using partitions. -/
+
+def IsPartitionGraph (G : Graph (Set α) β) : Prop :=
+  ∃ P : Partition (Set α), P.parts = G.V
+
+def Setify (G : Graph α β) : Graph (Set α) β :=
+  vxMap G ({·})
+
+def Setify.HasIsom (G : Graph α β) : G ≤↔ G.Setify :=
+  vxMap.HasIsom ({·}) singleton_injective.injOn
+
+lemma Setify.IsPartitionGraph (G : Graph α β) : G.Setify.IsPartitionGraph := by
+  use Partition.discrete G.V
+  ext x
+  simp [Partition.discrete, Setify]
+  refine exists_congr fun a => and_congr_right fun ha => ?_
+  revert x
+  rw [eq_iff_eq_cancel_right]
+  simp [ha]
+
+@[simps! vxSet edgeSet]
+def VxIdentification (G : Graph (Set α) β) (P : Partition (Set (Set α))) :
+    Graph (Set α) β :=
+  G.vxMap (⋃₀ P.partOf ·)
+
+variable {P : Partition (Set (Set α))} (hP : ⋃₀ P.parts = G.V)
+
+@[simp]
+lemma vxIdentification_inc₂ : (G.VxIdentification P).Inc₂ e x y ↔ ∃ x' y',
+    G.Inc₂ e x' y' ∧ ⋃₀ P.partOf x' = x ∧ ⋃₀ P.partOf y' = y := by
+  rw [VxIdentification, vxMap_inc₂]
+
+lemma vxIdentification_inc₂_toMultiset :
+    (G.VxIdentification P).Inc₂ e x y ↔ (G.toMultiset e).map (⋃₀ P.partOf ·) = {x, y} := by
+  rw [VxIdentification, vxMap_inc₂_toMultiset]
+
+@[simp]
+lemma vxIdentification_toMultiset :
+    (G.VxIdentification P).toMultiset e = (G.toMultiset e).map (⋃₀ P.partOf ·) := by
+  rw [VxIdentification, vxMap_toMultiset]
+
+@[simp]
+lemma vxIdentification_inc : (G.VxIdentification P).Inc e x ↔ ∃ y, G.Inc e y ∧ ⋃₀ P.partOf y = x := by
+  rw [VxIdentification, vxMap_inc]
+
