Kura/Prop7_2_1.lean
@@ -1,0 +1,3 @@
+import Kura.Operation.Minor2
+
+
